src/Coinductive_Prop.thy
@@ -10,14 +10,14 @@ section \<open>Stepwise denotational interpretation of TESL atoms\<close>
 (* Denotational interpretation of TESL bounded by index *)
 fun TESL_interpretation_atomic_stepwise
     :: "('\<tau>::linordered_field) TESL_atomic \<Rightarrow> nat \<Rightarrow> '\<tau> run set" ("\<lbrakk> _ \<rbrakk>\<^sub>T\<^sub>E\<^sub>S\<^sub>L\<^bsup>\<ge> _\<^esup>") where
-    "\<lbrakk> K\<^sub>1 sporadic \<lfloor>\<tau>\<rfloor> on K\<^sub>2 \<rbrakk>\<^sub>T\<^sub>E\<^sub>S\<^sub>L\<^bsup>\<ge> i\<^esup> =
+    "\<lbrakk> K\<^sub>1 sporadic \<lparr>\<tau>\<rparr> on K\<^sub>2 \<rbrakk>\<^sub>T\<^sub>E\<^sub>S\<^sub>L\<^bsup>\<ge> i\<^esup> =
         { \<rho>. \<exists>n\<ge>i. hamlet ((Rep_run \<rho>) n K\<^sub>1) = True \<and> time ((Rep_run \<rho>) n K\<^sub>2) = \<tau> }"
-  | "\<lbrakk> K\<^sub>1 sporadic \<lfloor>\<tau>\<^sub>v\<^sub>a\<^sub>r(K\<^sub>p\<^sub>a\<^sub>s\<^sub>t, n\<^sub>p\<^sub>a\<^sub>s\<^sub>t) \<oplus> \<delta>\<tau>\<rfloor> on K\<^sub>2 \<rbrakk>\<^sub>T\<^sub>E\<^sub>S\<^sub>L\<^bsup>\<ge> i\<^esup> =
+  | "\<lbrakk> K\<^sub>1 sporadic \<lparr>\<tau>\<^sub>v\<^sub>a\<^sub>r(K\<^sub>p\<^sub>a\<^sub>s\<^sub>t, n\<^sub>p\<^sub>a\<^sub>s\<^sub>t) \<oplus> \<delta>\<tau>\<rparr> on K\<^sub>2 \<rbrakk>\<^sub>T\<^sub>E\<^sub>S\<^sub>L\<^bsup>\<ge> i\<^esup> =
         { \<rho>. \<exists>n\<ge>i. hamlet ((Rep_run \<rho>) n K\<^sub>1) = True
                          \<and> time ((Rep_run \<rho>) n K\<^sub>2) = time ((Rep_run \<rho>) n\<^sub>p\<^sub>a\<^sub>s\<^sub>t K\<^sub>p\<^sub>a\<^sub>s\<^sub>t) + \<delta>\<tau> }"
   (* | "\<lbrakk> tag-relation K\<^sub>1 = \<alpha> * K\<^sub>2 + \<beta> \<rbrakk>\<^sub>T\<^sub>E\<^sub>S\<^sub>L\<^bsup>\<ge> i\<^esup> =
         { \<rho>. \<forall>n\<ge>i. time ((Rep_run \<rho>) n K\<^sub>1) = \<alpha> * time ((Rep_run \<rho>) n K\<^sub>2) + \<beta> }" *)
-  | "\<lbrakk> tag-relation \<langle>K\<^sub>1, K\<^sub>2\<rangle> \<in> R \<rbrakk>\<^sub>T\<^sub>E\<^sub>S\<^sub>L\<^bsup>\<ge> i\<^esup> =
+  | "\<lbrakk> tag-relation \<lfloor>K\<^sub>1, K\<^sub>2\<rfloor> \<in> R \<rbrakk>\<^sub>T\<^sub>E\<^sub>S\<^sub>L\<^bsup>\<ge> i\<^esup> =
         { \<rho>. \<forall>n\<ge>i. R (time ((Rep_run \<rho>) n K\<^sub>1), time ((Rep_run \<rho>) n K\<^sub>2)) }"
   | "\<lbrakk> master implies slave \<rbrakk>\<^sub>T\<^sub>E\<^sub>S\<^sub>L\<^bsup>\<ge> i\<^esup> =
         { \<rho>. \<forall>n\<ge>i. hamlet ((Rep_run \<rho>) n master) \<longrightarrow> hamlet ((Rep_run \<rho>) n slave) }"
@@ -42,11 +42,11 @@ theorem predicate_Union_unfold:
   by auto
 
 lemma TESL_interp_unfold_stepwise_sporadicon:
-  shows "\<lbrakk> K\<^sub>1 sporadic \<lfloor>\<tau>\<rfloor> on K\<^sub>2 \<rbrakk>\<^sub>T\<^sub>E\<^sub>S\<^sub>L = \<Union> {Y. \<exists>n::nat. Y = \<lbrakk> K\<^sub>1 sporadic \<lfloor>\<tau>\<rfloor> on K\<^sub>2 \<rbrakk>\<^sub>T\<^sub>E\<^sub>S\<^sub>L\<^bsup>\<ge> n\<^esup>}"
+  shows "\<lbrakk> K\<^sub>1 sporadic \<lparr>\<tau>\<rparr> on K\<^sub>2 \<rbrakk>\<^sub>T\<^sub>E\<^sub>S\<^sub>L = \<Union> {Y. \<exists>n::nat. Y = \<lbrakk> K\<^sub>1 sporadic \<lparr>\<tau>\<rparr> on K\<^sub>2 \<rbrakk>\<^sub>T\<^sub>E\<^sub>S\<^sub>L\<^bsup>\<ge> n\<^esup>}"
   by auto
 
 lemma TESL_interp_unfold_stepwise_sporadicon_add:
-  shows "\<lbrakk> K\<^sub>1 sporadic \<lfloor>\<tau>\<^sub>v\<^sub>a\<^sub>r(K, n') \<oplus> \<tau>\<rfloor> on K\<^sub>2 \<rbrakk>\<^sub>T\<^sub>E\<^sub>S\<^sub>L = \<Union> {Y. \<exists>n::nat. Y = \<lbrakk> K\<^sub>1 sporadic \<lfloor>\<tau>\<^sub>v\<^sub>a\<^sub>r(K, n') \<oplus> \<tau>\<rfloor> on K\<^sub>2 \<rbrakk>\<^sub>T\<^sub>E\<^sub>S\<^sub>L\<^bsup>\<ge> n\<^esup>}"
+  shows "\<lbrakk> K\<^sub>1 sporadic \<lparr>\<tau>\<^sub>v\<^sub>a\<^sub>r(K, n') \<oplus> \<tau>\<rparr> on K\<^sub>2 \<rbrakk>\<^sub>T\<^sub>E\<^sub>S\<^sub>L = \<Union> {Y. \<exists>n::nat. Y = \<lbrakk> K\<^sub>1 sporadic \<lparr>\<tau>\<^sub>v\<^sub>a\<^sub>r(K, n') \<oplus> \<tau>\<rparr> on K\<^sub>2 \<rbrakk>\<^sub>T\<^sub>E\<^sub>S\<^sub>L\<^bsup>\<ge> n\<^esup>}"
   by auto
 
 (*
@@ -56,7 +56,7 @@ lemma TESL_interp_unfold_stepwise_tagrel:
 *)
 
 lemma TESL_interp_unfold_stepwise_tagrelgen:
-  shows "\<lbrakk> tag-relation \<langle>K\<^sub>1, K\<^sub>2\<rangle> \<in> R \<rbrakk>\<^sub>T\<^sub>E\<^sub>S\<^sub>L = \<Inter> {Y. \<exists>n::nat. Y = \<lbrakk> tag-relation \<langle>K\<^sub>1, K\<^sub>2\<rangle> \<in> R \<rbrakk>\<^sub>T\<^sub>E\<^sub>S\<^sub>L\<^bsup>\<ge> n\<^esup>}"
+  shows "\<lbrakk> tag-relation \<lfloor>K\<^sub>1, K\<^sub>2\<rfloor> \<in> R \<rbrakk>\<^sub>T\<^sub>E\<^sub>S\<^sub>L = \<Inter> {Y. \<exists>n::nat. Y = \<lbrakk> tag-relation \<lfloor>K\<^sub>1, K\<^sub>2\<rfloor> \<in> R \<rbrakk>\<^sub>T\<^sub>E\<^sub>S\<^sub>L\<^bsup>\<ge> n\<^esup>}"
   by auto
 
 lemma TESL_interp_unfold_stepwise_implies:
@@ -79,21 +79,15 @@ lemma TESL_interp_unfold_stepwise_precedes:
 theorem TESL_interp_unfold_stepwise_positive_atoms:
   assumes "positive_atom \<phi>"
   shows "\<lbrakk> \<phi>::'\<tau>::linordered_field TESL_atomic \<rbrakk>\<^sub>T\<^sub>E\<^sub>S\<^sub>L = \<Union> {Y. \<exists>n::nat. Y = \<lbrakk> \<phi> \<rbrakk>\<^sub>T\<^sub>E\<^sub>S\<^sub>L\<^bsup>\<ge> n\<^esup>}"
-  sorry
-(*
   proof -
-    obtain cc :: "'\<tau> TESL_atomic \<Rightarrow> clock" and tt :: "'\<tau> TESL_atomic \<Rightarrow> '\<tau> tag_const" and cca :: "'\<tau> TESL_atomic \<Rightarrow> clock" and tta :: "'\<tau> TESL_atomic \<Rightarrow> '\<tau> tag_expr" and ccb :: "'\<tau> TESL_atomic \<Rightarrow> clock" where
-      f1: "(cca \<phi> sporadic tta \<phi> on ccb \<phi>) = \<phi> \<or> cc \<phi> sporadic tt \<phi> = \<phi>"
-      by (metis (no_types) assms positive_atom.elims(2))
-    { assume "\<Union>{R. \<exists>n. R = \<lbrakk> \<phi> \<rbrakk>\<^sub>T\<^sub>E\<^sub>S\<^sub>L\<^bsup>\<ge> n\<^esup>} \<noteq> \<lbrakk> \<phi> \<rbrakk>\<^sub>T\<^sub>E\<^sub>S\<^sub>L"
-      then have "cc \<phi> sporadic tt \<phi> \<noteq> \<phi>"
-        by (metis TESL_interp_unfold_stepwise_sporadic)
-      then have ?thesis
-        using f1 by (metis (no_types) TESL_interp_unfold_stepwise_sporadicon TESL_interp_unfold_stepwise_sporadicon_add old.prod.exhaust tag_expr.exhaust tag_var.exhaust) }
+    have "\<forall>t p c ca. \<Union>{R. \<exists>n. R = \<lbrakk> ca sporadic \<lparr> \<tau>\<^sub>v\<^sub>a\<^sub>r p \<oplus> t::'\<tau> tag_const \<rparr> on c \<rbrakk>\<^sub>T\<^sub>E\<^sub>S\<^sub>L\<^bsup>\<ge> n\<^esup>} = \<lbrakk> ca sporadic \<lparr> \<tau>\<^sub>v\<^sub>a\<^sub>r p \<oplus> t \<rparr> on c \<rbrakk>\<^sub>T\<^sub>E\<^sub>S\<^sub>L"
+      by auto
+    then obtain tt :: "'\<tau> tag_expr \<Rightarrow> '\<tau> tag_const" where
+      "\<forall>c ca t. \<Union>{R. \<exists>n. R = \<lbrakk> c sporadic t on ca \<rbrakk>\<^sub>T\<^sub>E\<^sub>S\<^sub>L\<^bsup>\<ge> n\<^esup>} = \<lbrakk> c sporadic t on ca \<rbrakk>\<^sub>T\<^sub>E\<^sub>S\<^sub>L \<or> \<lparr> tt t \<rparr> = t"
+      by (metis tag_expr.exhaust tag_var.exhaust)
     then show ?thesis
-      by blast
+      by (metis (no_types) TESL_interp_unfold_stepwise_sporadicon assms positive_atom.elims(2))
   qed
-*)
 
 theorem TESL_interp_unfold_stepwise_negative_atoms:
   assumes "\<not> positive_atom \<phi>"
@@ -140,9 +134,9 @@ qed
 section \<open>Coinduction unfolding properties\<close>
 
 lemma TESL_interp_stepwise_sporadicon_cst_coind_unfold:
-  shows "\<lbrakk> K\<^sub>1 sporadic \<lfloor>\<tau>\<rfloor> on K\<^sub>2 \<rbrakk>\<^sub>T\<^sub>E\<^sub>S\<^sub>L\<^bsup>\<ge> n\<^esup> =
-    \<lbrakk> K\<^sub>1 \<Up> n \<rbrakk>\<^sub>p\<^sub>r\<^sub>i\<^sub>m \<inter> \<lbrakk> K\<^sub>2 \<Down> n @ \<lfloor> \<tau> \<rfloor> \<rbrakk>\<^sub>p\<^sub>r\<^sub>i\<^sub>m
-    \<union> \<lbrakk> K\<^sub>1 sporadic \<lfloor>\<tau>\<rfloor> on K\<^sub>2 \<rbrakk>\<^sub>T\<^sub>E\<^sub>S\<^sub>L\<^bsup>\<ge> Suc n\<^esup>"
+  shows "\<lbrakk> K\<^sub>1 sporadic \<lparr>\<tau>\<rparr> on K\<^sub>2 \<rbrakk>\<^sub>T\<^sub>E\<^sub>S\<^sub>L\<^bsup>\<ge> n\<^esup> =
+    \<lbrakk> K\<^sub>1 \<Up> n \<rbrakk>\<^sub>p\<^sub>r\<^sub>i\<^sub>m \<inter> \<lbrakk> K\<^sub>2 \<Down> n @ \<lparr> \<tau> \<rparr> \<rbrakk>\<^sub>p\<^sub>r\<^sub>i\<^sub>m
+    \<union> \<lbrakk> K\<^sub>1 sporadic \<lparr>\<tau>\<rparr> on K\<^sub>2 \<rbrakk>\<^sub>T\<^sub>E\<^sub>S\<^sub>L\<^bsup>\<ge> Suc n\<^esup>"
   proof -
     have "{ \<rho>. \<exists>m\<ge>n. hamlet ((Rep_run \<rho>) m K\<^sub>1) = True \<and> time ((Rep_run \<rho>) m K\<^sub>2) = \<tau> }
         = { \<rho>. hamlet ((Rep_run \<rho>) n K\<^sub>1) = True \<and> time ((Rep_run \<rho>) n K\<^sub>2) = \<tau>
@@ -150,15 +144,15 @@ lemma TESL_interp_stepwise_sporadicon_cst_coind_unfold:
       using Suc_leD not_less_eq_eq by fastforce
     moreover have "{ \<rho>. hamlet ((Rep_run \<rho>) n K\<^sub>1) = True \<and> time ((Rep_run \<rho>) n K\<^sub>2) = \<tau>
                         \<or> (\<exists>m\<ge>Suc n. hamlet ((Rep_run \<rho>) m K\<^sub>1) = True \<and> time ((Rep_run \<rho>) m K\<^sub>2) = \<tau>) }
-                 = \<lbrakk> K\<^sub>1 \<Up> n \<rbrakk>\<^sub>p\<^sub>r\<^sub>i\<^sub>m \<inter> \<lbrakk> K\<^sub>2 \<Down> n @ \<lfloor>\<tau>\<rfloor> \<rbrakk>\<^sub>p\<^sub>r\<^sub>i\<^sub>m \<union> \<lbrakk> K\<^sub>1 sporadic \<lfloor>\<tau>\<rfloor> on K\<^sub>2 \<rbrakk>\<^sub>T\<^sub>E\<^sub>S\<^sub>L\<^bsup>\<ge> Suc n\<^esup>"
+                 = \<lbrakk> K\<^sub>1 \<Up> n \<rbrakk>\<^sub>p\<^sub>r\<^sub>i\<^sub>m \<inter> \<lbrakk> K\<^sub>2 \<Down> n @ \<lparr>\<tau>\<rparr> \<rbrakk>\<^sub>p\<^sub>r\<^sub>i\<^sub>m \<union> \<lbrakk> K\<^sub>1 sporadic \<lparr>\<tau>\<rparr> on K\<^sub>2 \<rbrakk>\<^sub>T\<^sub>E\<^sub>S\<^sub>L\<^bsup>\<ge> Suc n\<^esup>"
       by (simp add: Collect_conj_eq Collect_disj_eq)
     ultimately show ?thesis by auto
   qed
 
 lemma TESL_interp_stepwise_sporadicon_add_coind_unfold:
-  shows "\<lbrakk> K\<^sub>1 sporadic \<lfloor>\<tau>\<^sub>v\<^sub>a\<^sub>r(K, n') \<oplus> \<tau>\<rfloor> on K\<^sub>2 \<rbrakk>\<^sub>T\<^sub>E\<^sub>S\<^sub>L\<^bsup>\<ge> n\<^esup> =
-    \<lbrakk> K\<^sub>1 \<Up> n \<rbrakk>\<^sub>p\<^sub>r\<^sub>i\<^sub>m \<inter> \<lbrakk> K\<^sub>2 \<Down> n @ \<lfloor>\<tau>\<^sub>v\<^sub>a\<^sub>r(K, n') \<oplus> \<tau>\<rfloor> \<rbrakk>\<^sub>p\<^sub>r\<^sub>i\<^sub>m
-    \<union> \<lbrakk> K\<^sub>1 sporadic \<lfloor>\<tau>\<^sub>v\<^sub>a\<^sub>r(K, n') \<oplus> \<tau>\<rfloor> on K\<^sub>2 \<rbrakk>\<^sub>T\<^sub>E\<^sub>S\<^sub>L\<^bsup>\<ge> Suc n\<^esup>"
+  shows "\<lbrakk> K\<^sub>1 sporadic \<lparr>\<tau>\<^sub>v\<^sub>a\<^sub>r(K, n') \<oplus> \<tau>\<rparr> on K\<^sub>2 \<rbrakk>\<^sub>T\<^sub>E\<^sub>S\<^sub>L\<^bsup>\<ge> n\<^esup> =
+    \<lbrakk> K\<^sub>1 \<Up> n \<rbrakk>\<^sub>p\<^sub>r\<^sub>i\<^sub>m \<inter> \<lbrakk> K\<^sub>2 \<Down> n @ \<lparr>\<tau>\<^sub>v\<^sub>a\<^sub>r(K, n') \<oplus> \<tau>\<rparr> \<rbrakk>\<^sub>p\<^sub>r\<^sub>i\<^sub>m
+    \<union> \<lbrakk> K\<^sub>1 sporadic \<lparr>\<tau>\<^sub>v\<^sub>a\<^sub>r(K, n') \<oplus> \<tau>\<rparr> on K\<^sub>2 \<rbrakk>\<^sub>T\<^sub>E\<^sub>S\<^sub>L\<^bsup>\<ge> Suc n\<^esup>"
   proof -
     have "{ \<rho>. \<exists>m\<ge>n. hamlet ((Rep_run \<rho>) m K\<^sub>1) = True \<and> time ((Rep_run \<rho>) m K\<^sub>2) = time ((Rep_run \<rho>) n' K) + \<tau> }
         = { \<rho>. hamlet ((Rep_run \<rho>) n K\<^sub>1) = True \<and> time ((Rep_run \<rho>) n K\<^sub>2) = time ((Rep_run \<rho>) n' K) + \<tau>
@@ -178,7 +172,7 @@ lemma TESL_interp_stepwise_sporadicon_coind_unfold:
     case (AddDelay tagv x2)
     then show ?case
       proof (induct tagv)
-        case (Schematic xa)
+        case (TSchematic xa)
         then show ?case
           proof (induct xa)
             case (Pair a b)
@@ -220,9 +214,9 @@ lemma TESL_interp_stepwise_tagrelaff_coind_unfold:
 *)
 
 lemma TESL_interp_stepwise_tagrel_coind_unfold:
-  shows "\<lbrakk> tag-relation \<langle>K\<^sub>1, K\<^sub>2\<rangle> \<in> R \<rbrakk>\<^sub>T\<^sub>E\<^sub>S\<^sub>L\<^bsup>\<ge> n\<^esup> =
-    \<lbrakk> \<langle>\<tau>\<^sub>v\<^sub>a\<^sub>r(K\<^sub>1, n), \<tau>\<^sub>v\<^sub>a\<^sub>r(K\<^sub>2, n)\<rangle> \<in> R \<rbrakk>\<^sub>p\<^sub>r\<^sub>i\<^sub>m
-    \<inter> \<lbrakk> tag-relation \<langle>K\<^sub>1, K\<^sub>2\<rangle> \<in> R \<rbrakk>\<^sub>T\<^sub>E\<^sub>S\<^sub>L\<^bsup>\<ge> Suc n\<^esup>"
+  shows "\<lbrakk> tag-relation \<lfloor>K\<^sub>1, K\<^sub>2\<rfloor> \<in> R \<rbrakk>\<^sub>T\<^sub>E\<^sub>S\<^sub>L\<^bsup>\<ge> n\<^esup> =
+    \<lbrakk> \<lfloor>\<tau>\<^sub>v\<^sub>a\<^sub>r(K\<^sub>1, n), \<tau>\<^sub>v\<^sub>a\<^sub>r(K\<^sub>2, n)\<rfloor> \<in> R \<rbrakk>\<^sub>p\<^sub>r\<^sub>i\<^sub>m
+    \<inter> \<lbrakk> tag-relation \<lfloor>K\<^sub>1, K\<^sub>2\<rfloor> \<in> R \<rbrakk>\<^sub>T\<^sub>E\<^sub>S\<^sub>L\<^bsup>\<ge> Suc n\<^esup>"
   proof -
     have "{ \<rho>. \<forall>m\<ge>n. R (time ((Rep_run \<rho>) m K\<^sub>1), time ((Rep_run \<rho>) m K\<^sub>2)) }
          = { \<rho>. R (time ((Rep_run \<rho>) n K\<^sub>1), time ((Rep_run \<rho>) n K\<^sub>2)) }
@@ -243,9 +237,21 @@ lemma TESL_interp_stepwise_implies_coind_unfold:
     then show ?thesis by auto
   qed
 
+lemma TESL_interp_stepwise_implies_not_coind_unfold:
+  shows "\<lbrakk> master implies not slave \<rbrakk>\<^sub>T\<^sub>E\<^sub>S\<^sub>L\<^bsup>\<ge> n\<^esup> =
+    (\<lbrakk> master \<not>\<Up> n \<rbrakk>\<^sub>p\<^sub>r\<^sub>i\<^sub>m \<union> \<lbrakk> master \<Up> n \<rbrakk>\<^sub>p\<^sub>r\<^sub>i\<^sub>m \<inter> \<lbrakk> slave \<not>\<Up> n \<rbrakk>\<^sub>p\<^sub>r\<^sub>i\<^sub>m)
+    \<inter> \<lbrakk> master implies not slave \<rbrakk>\<^sub>T\<^sub>E\<^sub>S\<^sub>L\<^bsup>\<ge> Suc n\<^esup>"
+  proof -
+    have "{ \<rho>. \<forall>m\<ge>n. hamlet ((Rep_run \<rho>) m master) \<longrightarrow> \<not> hamlet ((Rep_run \<rho>) m slave) }
+          = { \<rho>. hamlet ((Rep_run \<rho>) n master) \<longrightarrow> \<not> hamlet ((Rep_run \<rho>) n slave) }
+          \<inter> { \<rho>. \<forall>m\<ge>Suc n. hamlet ((Rep_run \<rho>) m master) \<longrightarrow> \<not> hamlet ((Rep_run \<rho>) m slave) }"
+      using nat_set_suc[of "n" "\<lambda>x y. hamlet ((Rep_run x) y master) \<longrightarrow> \<not> hamlet ((Rep_run x) y slave)"] by simp
+    then show ?thesis by auto
+  qed
+
 lemma TESL_interp_stepwise_timedelayed_coind_unfold:
   shows "\<lbrakk> master time-delayed by \<delta>\<tau> on measuring implies slave \<rbrakk>\<^sub>T\<^sub>E\<^sub>S\<^sub>L\<^bsup>\<ge> n\<^esup> =
-    (\<lbrakk> master \<not>\<Up> n \<rbrakk>\<^sub>p\<^sub>r\<^sub>i\<^sub>m \<union> \<lbrakk> master \<Up> n \<rbrakk>\<^sub>p\<^sub>r\<^sub>i\<^sub>m \<inter> \<lbrakk> slave sporadic \<lfloor>\<tau>\<^sub>v\<^sub>a\<^sub>r(measuring, n) \<oplus> \<delta>\<tau>\<rfloor> on measuring \<rbrakk>\<^sub>T\<^sub>E\<^sub>S\<^sub>L\<^bsup>\<ge> n\<^esup>)
+    (\<lbrakk> master \<not>\<Up> n \<rbrakk>\<^sub>p\<^sub>r\<^sub>i\<^sub>m \<union> \<lbrakk> master \<Up> n \<rbrakk>\<^sub>p\<^sub>r\<^sub>i\<^sub>m \<inter> \<lbrakk> slave sporadic \<lparr>\<tau>\<^sub>v\<^sub>a\<^sub>r(measuring, n) \<oplus> \<delta>\<tau>\<rparr> on measuring \<rbrakk>\<^sub>T\<^sub>E\<^sub>S\<^sub>L\<^bsup>\<ge> n\<^esup>)
     \<inter> \<lbrakk> master time-delayed by \<delta>\<tau> on measuring implies slave \<rbrakk>\<^sub>T\<^sub>E\<^sub>S\<^sub>L\<^bsup>\<ge> Suc n\<^esup>"
   proof -
     have "{ \<rho>. \<forall>m\<ge>n. hamlet ((Rep_run \<rho>) m master) \<longrightarrow>
@@ -265,9 +271,16 @@ lemma TESL_interp_stepwise_timedelayed_coind_unfold:
 
 lemma TESL_interp_stepwise_precedes_coind_unfold:
   shows "\<lbrakk> K\<^sub>1 precedes K\<^sub>2 \<rbrakk>\<^sub>T\<^sub>E\<^sub>S\<^sub>L\<^bsup>\<ge> n\<^esup> =
-    (\<lbrakk> (#\<^sup>\<le> K\<^sub>2 n) \<preceq> (#\<^sup>< K\<^sub>1 n) \<rbrakk>\<^sub>p\<^sub>r\<^sub>i\<^sub>m)
+    \<lbrakk> (\<lceil>#\<^sup>\<le> K\<^sub>2 n, #\<^sup>< K\<^sub>1 n\<rceil> \<in> (\<lambda>(x,y). x\<le>y)) \<rbrakk>\<^sub>p\<^sub>r\<^sub>i\<^sub>m
     \<inter> \<lbrakk> K\<^sub>1 precedes K\<^sub>2 \<rbrakk>\<^sub>T\<^sub>E\<^sub>S\<^sub>L\<^bsup>\<ge> Suc n\<^esup>"
-  sorry
+  proof -
+    have "{ \<rho>. \<forall>p\<ge>n. (run_tick_count \<rho> K\<^sub>2 p) \<le> (run_tick_count_strictly \<rho> K\<^sub>1 p) }
+           = { \<rho>. (run_tick_count \<rho> K\<^sub>2 n) \<le> (run_tick_count_strictly \<rho> K\<^sub>1 n) }
+           \<inter> { \<rho>. \<forall>p\<ge>Suc n. (run_tick_count \<rho> K\<^sub>2 p) \<le> (run_tick_count_strictly \<rho> K\<^sub>1 p) }"
+      using nat_set_suc[of "n" "\<lambda>\<rho> n. (run_tick_count \<rho> K\<^sub>2 n) \<le> (run_tick_count_strictly \<rho> K\<^sub>1 n)"]
+      by simp
+    then show ?thesis by auto
+  qed
 
 fun TESL_interpretation_stepwise :: "'\<tau>::linordered_field TESL_formula \<Rightarrow> nat \<Rightarrow> '\<tau> run set" ("\<lbrakk>\<lbrakk> _ \<rbrakk>\<rbrakk>\<^sub>T\<^sub>E\<^sub>S\<^sub>L\<^bsup>\<ge> _\<^esup>") where
     "\<lbrakk>\<lbrakk> [] \<rbrakk>\<rbrakk>\<^sub>T\<^sub>E\<^sub>S\<^sub>L\<^bsup>\<ge> n\<^esup> = { _. True }"
@@ -295,7 +308,7 @@ lemma TESL_interpretation_stepwise_zero:
         case (AddDelay tag x2)
         then show ?case
           proof (induct tag)
-            case (Schematic xa)
+            case (TSchematic xa)
             then show ?case
               proof (induct xa)
                 case (Pair a b)
@@ -319,6 +332,9 @@ lemma TESL_interpretation_stepwise_zero:
     then show ?case by simp
   next
     case (TimeDelayedBy x1 x2 x3 x4)
+    then show ?case by simp
+  next
+    case (Precedes x1 x2)
     then show ?case by simp
   qed
 
@@ -415,17 +431,17 @@ lemma HeronConf_interp_stepwise_tagrelaff_cases:
 *)
 
 lemma HeronConf_interp_stepwise_tagrel_cases:
-  shows "\<lbrakk> \<Gamma>, n \<turnstile> ((tag-relation \<langle>K\<^sub>1, K\<^sub>2\<rangle> \<in> R) # \<Psi>) \<triangleright> \<Phi> \<rbrakk>\<^sub>c\<^sub>o\<^sub>n\<^sub>f\<^sub>i\<^sub>g
-          = \<lbrakk> ((\<langle>\<tau>\<^sub>v\<^sub>a\<^sub>r(K\<^sub>1, n), \<tau>\<^sub>v\<^sub>a\<^sub>r(K\<^sub>2, n)\<rangle> \<in> R) # \<Gamma>), n \<turnstile> \<Psi> \<triangleright> ((tag-relation \<langle>K\<^sub>1, K\<^sub>2\<rangle> \<in> R) # \<Phi>) \<rbrakk>\<^sub>c\<^sub>o\<^sub>n\<^sub>f\<^sub>i\<^sub>g"
+  shows "\<lbrakk> \<Gamma>, n \<turnstile> ((tag-relation \<lfloor>K\<^sub>1, K\<^sub>2\<rfloor> \<in> R) # \<Psi>) \<triangleright> \<Phi> \<rbrakk>\<^sub>c\<^sub>o\<^sub>n\<^sub>f\<^sub>i\<^sub>g
+          = \<lbrakk> ((\<lfloor>\<tau>\<^sub>v\<^sub>a\<^sub>r(K\<^sub>1, n), \<tau>\<^sub>v\<^sub>a\<^sub>r(K\<^sub>2, n)\<rfloor> \<in> R) # \<Gamma>), n \<turnstile> \<Psi> \<triangleright> ((tag-relation \<lfloor>K\<^sub>1, K\<^sub>2\<rfloor> \<in> R) # \<Phi>) \<rbrakk>\<^sub>c\<^sub>o\<^sub>n\<^sub>f\<^sub>i\<^sub>g"
   proof -
-    have "\<lbrakk> \<Gamma>, n \<turnstile> (tag-relation \<langle>K\<^sub>1, K\<^sub>2\<rangle> \<in> R) # \<Psi> \<triangleright> \<Phi> \<rbrakk>\<^sub>c\<^sub>o\<^sub>n\<^sub>f\<^sub>i\<^sub>g = \<lbrakk>\<lbrakk> \<Gamma> \<rbrakk>\<rbrakk>\<^sub>p\<^sub>r\<^sub>i\<^sub>m \<inter> \<lbrakk>\<lbrakk> (tag-relation \<langle>K\<^sub>1, K\<^sub>2\<rangle> \<in> R) # \<Psi> \<rbrakk>\<rbrakk>\<^sub>T\<^sub>E\<^sub>S\<^sub>L\<^bsup>\<ge> n\<^esup> \<inter> \<lbrakk>\<lbrakk> \<Phi> \<rbrakk>\<rbrakk>\<^sub>T\<^sub>E\<^sub>S\<^sub>L\<^bsup>\<ge> Suc n\<^esup>"
+    have "\<lbrakk> \<Gamma>, n \<turnstile> (tag-relation \<lfloor>K\<^sub>1, K\<^sub>2\<rfloor> \<in> R) # \<Psi> \<triangleright> \<Phi> \<rbrakk>\<^sub>c\<^sub>o\<^sub>n\<^sub>f\<^sub>i\<^sub>g = \<lbrakk>\<lbrakk> \<Gamma> \<rbrakk>\<rbrakk>\<^sub>p\<^sub>r\<^sub>i\<^sub>m \<inter> \<lbrakk>\<lbrakk> (tag-relation \<lfloor>K\<^sub>1, K\<^sub>2\<rfloor> \<in> R) # \<Psi> \<rbrakk>\<rbrakk>\<^sub>T\<^sub>E\<^sub>S\<^sub>L\<^bsup>\<ge> n\<^esup> \<inter> \<lbrakk>\<lbrakk> \<Phi> \<rbrakk>\<rbrakk>\<^sub>T\<^sub>E\<^sub>S\<^sub>L\<^bsup>\<ge> Suc n\<^esup>"
       by simp
-    moreover have "\<lbrakk> ((\<langle>\<tau>\<^sub>v\<^sub>a\<^sub>r(K\<^sub>1, n), \<tau>\<^sub>v\<^sub>a\<^sub>r(K\<^sub>2, n)\<rangle> \<in> R) # \<Gamma>), n \<turnstile> \<Psi> \<triangleright> ((tag-relation \<langle>K\<^sub>1, K\<^sub>2\<rangle> \<in> R) # \<Phi>) \<rbrakk>\<^sub>c\<^sub>o\<^sub>n\<^sub>f\<^sub>i\<^sub>g
-                      = \<lbrakk>\<lbrakk> (\<langle>\<tau>\<^sub>v\<^sub>a\<^sub>r(K\<^sub>1, n), \<tau>\<^sub>v\<^sub>a\<^sub>r(K\<^sub>2, n)\<rangle> \<in> R) # \<Gamma> \<rbrakk>\<rbrakk>\<^sub>p\<^sub>r\<^sub>i\<^sub>m \<inter> \<lbrakk>\<lbrakk> \<Psi> \<rbrakk>\<rbrakk>\<^sub>T\<^sub>E\<^sub>S\<^sub>L\<^bsup>\<ge> n\<^esup> \<inter> \<lbrakk>\<lbrakk> (tag-relation \<langle>K\<^sub>1, K\<^sub>2\<rangle> \<in> R) # \<Phi> \<rbrakk>\<rbrakk>\<^sub>T\<^sub>E\<^sub>S\<^sub>L\<^bsup>\<ge> Suc n\<^esup>"
+    moreover have "\<lbrakk> ((\<lfloor>\<tau>\<^sub>v\<^sub>a\<^sub>r(K\<^sub>1, n), \<tau>\<^sub>v\<^sub>a\<^sub>r(K\<^sub>2, n)\<rfloor> \<in> R) # \<Gamma>), n \<turnstile> \<Psi> \<triangleright> ((tag-relation \<lfloor>K\<^sub>1, K\<^sub>2\<rfloor> \<in> R) # \<Phi>) \<rbrakk>\<^sub>c\<^sub>o\<^sub>n\<^sub>f\<^sub>i\<^sub>g
+                      = \<lbrakk>\<lbrakk> (\<lfloor>\<tau>\<^sub>v\<^sub>a\<^sub>r(K\<^sub>1, n), \<tau>\<^sub>v\<^sub>a\<^sub>r(K\<^sub>2, n)\<rfloor> \<in> R) # \<Gamma> \<rbrakk>\<rbrakk>\<^sub>p\<^sub>r\<^sub>i\<^sub>m \<inter> \<lbrakk>\<lbrakk> \<Psi> \<rbrakk>\<rbrakk>\<^sub>T\<^sub>E\<^sub>S\<^sub>L\<^bsup>\<ge> n\<^esup> \<inter> \<lbrakk>\<lbrakk> (tag-relation \<lfloor>K\<^sub>1, K\<^sub>2\<rfloor> \<in> R) # \<Phi> \<rbrakk>\<rbrakk>\<^sub>T\<^sub>E\<^sub>S\<^sub>L\<^bsup>\<ge> Suc n\<^esup>"
       by simp
     ultimately show ?thesis
     proof -
-      have "\<lbrakk> \<langle>\<tau>\<^sub>v\<^sub>a\<^sub>r(K\<^sub>1, n), \<tau>\<^sub>v\<^sub>a\<^sub>r(K\<^sub>2, n)\<rangle> \<in> R \<rbrakk>\<^sub>p\<^sub>r\<^sub>i\<^sub>m \<inter> \<lbrakk> tag-relation \<langle>K\<^sub>1, K\<^sub>2\<rangle> \<in> R \<rbrakk>\<^sub>T\<^sub>E\<^sub>S\<^sub>L\<^bsup>\<ge> Suc n\<^esup> \<inter> \<lbrakk>\<lbrakk> \<Psi> \<rbrakk>\<rbrakk>\<^sub>T\<^sub>E\<^sub>S\<^sub>L\<^bsup>\<ge> n\<^esup> = \<lbrakk>\<lbrakk> (tag-relation \<langle>K\<^sub>1, K\<^sub>2\<rangle> \<in> R) # \<Psi> \<rbrakk>\<rbrakk>\<^sub>T\<^sub>E\<^sub>S\<^sub>L\<^bsup>\<ge> n\<^esup>"
+      have "\<lbrakk> \<lfloor>\<tau>\<^sub>v\<^sub>a\<^sub>r(K\<^sub>1, n), \<tau>\<^sub>v\<^sub>a\<^sub>r(K\<^sub>2, n)\<rfloor> \<in> R \<rbrakk>\<^sub>p\<^sub>r\<^sub>i\<^sub>m \<inter> \<lbrakk> tag-relation \<lfloor>K\<^sub>1, K\<^sub>2\<rfloor> \<in> R \<rbrakk>\<^sub>T\<^sub>E\<^sub>S\<^sub>L\<^bsup>\<ge> Suc n\<^esup> \<inter> \<lbrakk>\<lbrakk> \<Psi> \<rbrakk>\<rbrakk>\<^sub>T\<^sub>E\<^sub>S\<^sub>L\<^bsup>\<ge> n\<^esup> = \<lbrakk>\<lbrakk> (tag-relation \<lfloor>K\<^sub>1, K\<^sub>2\<rfloor> \<in> R) # \<Psi> \<rbrakk>\<rbrakk>\<^sub>T\<^sub>E\<^sub>S\<^sub>L\<^bsup>\<ge> n\<^esup>"
         using TESL_interp_stepwise_tagrel_coind_unfold TESL_interpretation_stepwise_cons_morph by blast
       then show ?thesis
         by auto
@@ -460,12 +476,34 @@ lemma HeronConf_interp_stepwise_implies_not_cases:
   shows "\<lbrakk> \<Gamma>, n \<turnstile> ((K\<^sub>1 implies not K\<^sub>2) # \<Psi>) \<triangleright> \<Phi> \<rbrakk>\<^sub>c\<^sub>o\<^sub>n\<^sub>f\<^sub>i\<^sub>g
           = \<lbrakk> ((K\<^sub>1 \<not>\<Up> n) # \<Gamma>), n \<turnstile> \<Psi> \<triangleright> ((K\<^sub>1 implies not K\<^sub>2) # \<Phi>) \<rbrakk>\<^sub>c\<^sub>o\<^sub>n\<^sub>f\<^sub>i\<^sub>g
           \<union> \<lbrakk> ((K\<^sub>1 \<Up> n) # (K\<^sub>2 \<not>\<Up> n) # \<Gamma>), n \<turnstile> \<Psi> \<triangleright> ((K\<^sub>1 implies not K\<^sub>2) # \<Phi>) \<rbrakk>\<^sub>c\<^sub>o\<^sub>n\<^sub>f\<^sub>i\<^sub>g"
-  sorry
+  proof -
+    have "\<lbrakk> \<Gamma>, n \<turnstile> (K\<^sub>1 implies not K\<^sub>2) # \<Psi> \<triangleright> \<Phi> \<rbrakk>\<^sub>c\<^sub>o\<^sub>n\<^sub>f\<^sub>i\<^sub>g = \<lbrakk>\<lbrakk> \<Gamma> \<rbrakk>\<rbrakk>\<^sub>p\<^sub>r\<^sub>i\<^sub>m \<inter> \<lbrakk>\<lbrakk> (K\<^sub>1 implies not K\<^sub>2) # \<Psi> \<rbrakk>\<rbrakk>\<^sub>T\<^sub>E\<^sub>S\<^sub>L\<^bsup>\<ge> n\<^esup> \<inter> \<lbrakk>\<lbrakk> \<Phi> \<rbrakk>\<rbrakk>\<^sub>T\<^sub>E\<^sub>S\<^sub>L\<^bsup>\<ge> Suc n\<^esup>"
+      by simp
+    moreover have "\<lbrakk> ((K\<^sub>1 \<not>\<Up> n) # \<Gamma>), n \<turnstile> \<Psi> \<triangleright> ((K\<^sub>1 implies not K\<^sub>2) # \<Phi>) \<rbrakk>\<^sub>c\<^sub>o\<^sub>n\<^sub>f\<^sub>i\<^sub>g
+                      = \<lbrakk>\<lbrakk> (K\<^sub>1 \<not>\<Up> n) # \<Gamma> \<rbrakk>\<rbrakk>\<^sub>p\<^sub>r\<^sub>i\<^sub>m \<inter> \<lbrakk>\<lbrakk> \<Psi> \<rbrakk>\<rbrakk>\<^sub>T\<^sub>E\<^sub>S\<^sub>L\<^bsup>\<ge> n\<^esup> \<inter> \<lbrakk>\<lbrakk> (K\<^sub>1 implies not K\<^sub>2) # \<Phi> \<rbrakk>\<rbrakk>\<^sub>T\<^sub>E\<^sub>S\<^sub>L\<^bsup>\<ge> Suc n\<^esup>"
+      by simp
+    moreover have "\<lbrakk> ((K\<^sub>1 \<Up> n) # (K\<^sub>2 \<not>\<Up> n) # \<Gamma>), n \<turnstile> \<Psi> \<triangleright> ((K\<^sub>1 implies not K\<^sub>2) # \<Phi>) \<rbrakk>\<^sub>c\<^sub>o\<^sub>n\<^sub>f\<^sub>i\<^sub>g
+                      = \<lbrakk>\<lbrakk> ((K\<^sub>1 \<Up> n) # (K\<^sub>2 \<not>\<Up> n) # \<Gamma>) \<rbrakk>\<rbrakk>\<^sub>p\<^sub>r\<^sub>i\<^sub>m \<inter> \<lbrakk>\<lbrakk> \<Psi> \<rbrakk>\<rbrakk>\<^sub>T\<^sub>E\<^sub>S\<^sub>L\<^bsup>\<ge> n\<^esup> \<inter> \<lbrakk>\<lbrakk> (K\<^sub>1 implies not K\<^sub>2) # \<Phi> \<rbrakk>\<rbrakk>\<^sub>T\<^sub>E\<^sub>S\<^sub>L\<^bsup>\<ge> Suc n\<^esup>"
+      by simp
+    ultimately show ?thesis
+    proof -
+      have f1: "(\<lbrakk> K\<^sub>1 \<not>\<Up> n \<rbrakk>\<^sub>p\<^sub>r\<^sub>i\<^sub>m \<union> \<lbrakk> K\<^sub>1 \<Up> n \<rbrakk>\<^sub>p\<^sub>r\<^sub>i\<^sub>m \<inter> \<lbrakk> K\<^sub>2 \<not>\<Up> n \<rbrakk>\<^sub>p\<^sub>r\<^sub>i\<^sub>m) \<inter> \<lbrakk> K\<^sub>1 implies not K\<^sub>2 \<rbrakk>\<^sub>T\<^sub>E\<^sub>S\<^sub>L\<^bsup>\<ge> Suc n\<^esup> \<inter> (\<lbrakk>\<lbrakk> \<Psi> \<rbrakk>\<rbrakk>\<^sub>T\<^sub>E\<^sub>S\<^sub>L\<^bsup>\<ge> n\<^esup> \<inter> \<lbrakk>\<lbrakk> \<Phi> \<rbrakk>\<rbrakk>\<^sub>T\<^sub>E\<^sub>S\<^sub>L\<^bsup>\<ge> Suc n\<^esup>)
+                  = \<lbrakk>\<lbrakk> (K\<^sub>1 implies not K\<^sub>2) # \<Psi> \<rbrakk>\<rbrakk>\<^sub>T\<^sub>E\<^sub>S\<^sub>L\<^bsup>\<ge> n\<^esup> \<inter> \<lbrakk>\<lbrakk> \<Phi> \<rbrakk>\<rbrakk>\<^sub>T\<^sub>E\<^sub>S\<^sub>L\<^bsup>\<ge> Suc n\<^esup>"
+        using TESL_interp_stepwise_implies_not_coind_unfold TESL_interpretation_stepwise_cons_morph by blast
+      have "\<lbrakk> K\<^sub>1 \<not>\<Up> n \<rbrakk>\<^sub>p\<^sub>r\<^sub>i\<^sub>m \<inter> \<lbrakk>\<lbrakk> \<Gamma> \<rbrakk>\<rbrakk>\<^sub>p\<^sub>r\<^sub>i\<^sub>m \<union> \<lbrakk> K\<^sub>1 \<Up> n \<rbrakk>\<^sub>p\<^sub>r\<^sub>i\<^sub>m \<inter> \<lbrakk>\<lbrakk> (K\<^sub>2 \<not>\<Up> n) # \<Gamma> \<rbrakk>\<rbrakk>\<^sub>p\<^sub>r\<^sub>i\<^sub>m = (\<lbrakk> K\<^sub>1 \<not>\<Up> n \<rbrakk>\<^sub>p\<^sub>r\<^sub>i\<^sub>m \<union> \<lbrakk> K\<^sub>1 \<Up> n \<rbrakk>\<^sub>p\<^sub>r\<^sub>i\<^sub>m \<inter> \<lbrakk> K\<^sub>2 \<not>\<Up> n \<rbrakk>\<^sub>p\<^sub>r\<^sub>i\<^sub>m) \<inter> \<lbrakk>\<lbrakk> \<Gamma> \<rbrakk>\<rbrakk>\<^sub>p\<^sub>r\<^sub>i\<^sub>m"
+        by force
+      then have "\<lbrakk> \<Gamma>, n \<turnstile> ((K\<^sub>1 implies not K\<^sub>2) # \<Psi>) \<triangleright> \<Phi> \<rbrakk>\<^sub>c\<^sub>o\<^sub>n\<^sub>f\<^sub>i\<^sub>g
+                   = (\<lbrakk> K\<^sub>1 \<not>\<Up> n \<rbrakk>\<^sub>p\<^sub>r\<^sub>i\<^sub>m \<inter> \<lbrakk>\<lbrakk> \<Gamma> \<rbrakk>\<rbrakk>\<^sub>p\<^sub>r\<^sub>i\<^sub>m \<union> \<lbrakk> K\<^sub>1 \<Up> n \<rbrakk>\<^sub>p\<^sub>r\<^sub>i\<^sub>m \<inter> \<lbrakk>\<lbrakk> (K\<^sub>2 \<not>\<Up> n) # \<Gamma> \<rbrakk>\<rbrakk>\<^sub>p\<^sub>r\<^sub>i\<^sub>m) \<inter> (\<lbrakk>\<lbrakk> \<Psi> \<rbrakk>\<rbrakk>\<^sub>T\<^sub>E\<^sub>S\<^sub>L\<^bsup>\<ge> n\<^esup> \<inter> \<lbrakk>\<lbrakk> (K\<^sub>1 implies not K\<^sub>2) # \<Phi> \<rbrakk>\<rbrakk>\<^sub>T\<^sub>E\<^sub>S\<^sub>L\<^bsup>\<ge> Suc n\<^esup>)"
+        using f1 by (simp add: inf_left_commute inf_sup_aci(2))
+      then show ?thesis
+        by (simp add: Int_Un_distrib2 inf_sup_aci(2))
+    qed
+  qed
 
 lemma HeronConf_interp_stepwise_timedelayed_cases:
   shows "\<lbrakk> \<Gamma>, n \<turnstile> ((K\<^sub>1 time-delayed by \<delta>\<tau> on K\<^sub>2 implies K\<^sub>3) # \<Psi>) \<triangleright> \<Phi> \<rbrakk>\<^sub>c\<^sub>o\<^sub>n\<^sub>f\<^sub>i\<^sub>g
           = \<lbrakk> ((K\<^sub>1 \<not>\<Up> n) # \<Gamma>), n \<turnstile> \<Psi> \<triangleright> ((K\<^sub>1 time-delayed by \<delta>\<tau> on K\<^sub>2 implies K\<^sub>3) # \<Phi>) \<rbrakk>\<^sub>c\<^sub>o\<^sub>n\<^sub>f\<^sub>i\<^sub>g
-          \<union> \<lbrakk> ((K\<^sub>1 \<Up> n) # \<Gamma>), n \<turnstile> ((K\<^sub>3 sporadic \<lfloor>\<tau>\<^sub>v\<^sub>a\<^sub>r(K\<^sub>2, n) \<oplus> \<delta>\<tau>\<rfloor> on K\<^sub>2) # \<Psi>) \<triangleright> ((K\<^sub>1 time-delayed by \<delta>\<tau> on K\<^sub>2 implies K\<^sub>3) # \<Phi>) \<rbrakk>\<^sub>c\<^sub>o\<^sub>n\<^sub>f\<^sub>i\<^sub>g"
+          \<union> \<lbrakk> ((K\<^sub>1 \<Up> n) # \<Gamma>), n \<turnstile> ((K\<^sub>3 sporadic \<lparr>\<tau>\<^sub>v\<^sub>a\<^sub>r(K\<^sub>2, n) \<oplus> \<delta>\<tau>\<rparr> on K\<^sub>2) # \<Psi>) \<triangleright> ((K\<^sub>1 time-delayed by \<delta>\<tau> on K\<^sub>2 implies K\<^sub>3) # \<Phi>) \<rbrakk>\<^sub>c\<^sub>o\<^sub>n\<^sub>f\<^sub>i\<^sub>g"
   proof -
     have "\<lbrakk> \<Gamma>, n \<turnstile> (K\<^sub>1 time-delayed by \<delta>\<tau> on K\<^sub>2 implies K\<^sub>3) # \<Psi> \<triangleright> \<Phi> \<rbrakk>\<^sub>c\<^sub>o\<^sub>n\<^sub>f\<^sub>i\<^sub>g
            = \<lbrakk>\<lbrakk> \<Gamma> \<rbrakk>\<rbrakk>\<^sub>p\<^sub>r\<^sub>i\<^sub>m \<inter> \<lbrakk>\<lbrakk> (K\<^sub>1 time-delayed by \<delta>\<tau> on K\<^sub>2 implies K\<^sub>3) # \<Psi> \<rbrakk>\<rbrakk>\<^sub>T\<^sub>E\<^sub>S\<^sub>L\<^bsup>\<ge> n\<^esup> \<inter> \<lbrakk>\<lbrakk> \<Phi> \<rbrakk>\<rbrakk>\<^sub>T\<^sub>E\<^sub>S\<^sub>L\<^bsup>\<ge> Suc n\<^esup>"
@@ -473,25 +511,42 @@ lemma HeronConf_interp_stepwise_timedelayed_cases:
     moreover have "\<lbrakk> ((K\<^sub>1 \<not>\<Up> n) # \<Gamma>), n \<turnstile> \<Psi> \<triangleright> ((K\<^sub>1 time-delayed by \<delta>\<tau> on K\<^sub>2 implies K\<^sub>3) # \<Phi>) \<rbrakk>\<^sub>c\<^sub>o\<^sub>n\<^sub>f\<^sub>i\<^sub>g
                      = \<lbrakk>\<lbrakk> (K\<^sub>1 \<not>\<Up> n) # \<Gamma> \<rbrakk>\<rbrakk>\<^sub>p\<^sub>r\<^sub>i\<^sub>m \<inter> \<lbrakk>\<lbrakk> \<Psi> \<rbrakk>\<rbrakk>\<^sub>T\<^sub>E\<^sub>S\<^sub>L\<^bsup>\<ge> n\<^esup> \<inter> \<lbrakk>\<lbrakk> (K\<^sub>1 time-delayed by \<delta>\<tau> on K\<^sub>2 implies K\<^sub>3) # \<Phi> \<rbrakk>\<rbrakk>\<^sub>T\<^sub>E\<^sub>S\<^sub>L\<^bsup>\<ge> Suc n\<^esup>"
       by simp
-    moreover have "\<lbrakk> ((K\<^sub>1 \<Up> n) # \<Gamma>), n \<turnstile> ((K\<^sub>3 sporadic \<lfloor>\<tau>\<^sub>v\<^sub>a\<^sub>r(K\<^sub>2, n) \<oplus> \<delta>\<tau>\<rfloor> on K\<^sub>2) # \<Psi>) \<triangleright> ((K\<^sub>1 time-delayed by \<delta>\<tau> on K\<^sub>2 implies K\<^sub>3) # \<Phi>) \<rbrakk>\<^sub>c\<^sub>o\<^sub>n\<^sub>f\<^sub>i\<^sub>g
-                     = \<lbrakk>\<lbrakk> (K\<^sub>1 \<Up> n) # \<Gamma> \<rbrakk>\<rbrakk>\<^sub>p\<^sub>r\<^sub>i\<^sub>m \<inter> \<lbrakk>\<lbrakk> (K\<^sub>3 sporadic \<lfloor>\<tau>\<^sub>v\<^sub>a\<^sub>r(K\<^sub>2, n) \<oplus> \<delta>\<tau>\<rfloor> on K\<^sub>2) # \<Psi> \<rbrakk>\<rbrakk>\<^sub>T\<^sub>E\<^sub>S\<^sub>L\<^bsup>\<ge> n\<^esup>
+    moreover have "\<lbrakk> ((K\<^sub>1 \<Up> n) # \<Gamma>), n \<turnstile> ((K\<^sub>3 sporadic \<lparr>\<tau>\<^sub>v\<^sub>a\<^sub>r(K\<^sub>2, n) \<oplus> \<delta>\<tau>\<rparr> on K\<^sub>2) # \<Psi>) \<triangleright> ((K\<^sub>1 time-delayed by \<delta>\<tau> on K\<^sub>2 implies K\<^sub>3) # \<Phi>) \<rbrakk>\<^sub>c\<^sub>o\<^sub>n\<^sub>f\<^sub>i\<^sub>g
+                     = \<lbrakk>\<lbrakk> (K\<^sub>1 \<Up> n) # \<Gamma> \<rbrakk>\<rbrakk>\<^sub>p\<^sub>r\<^sub>i\<^sub>m \<inter> \<lbrakk>\<lbrakk> (K\<^sub>3 sporadic \<lparr>\<tau>\<^sub>v\<^sub>a\<^sub>r(K\<^sub>2, n) \<oplus> \<delta>\<tau>\<rparr> on K\<^sub>2) # \<Psi> \<rbrakk>\<rbrakk>\<^sub>T\<^sub>E\<^sub>S\<^sub>L\<^bsup>\<ge> n\<^esup>
                      \<inter> \<lbrakk>\<lbrakk> (K\<^sub>1 time-delayed by \<delta>\<tau> on K\<^sub>2 implies K\<^sub>3) # \<Phi> \<rbrakk>\<rbrakk>\<^sub>T\<^sub>E\<^sub>S\<^sub>L\<^bsup>\<ge> Suc n\<^esup>"
       by simp
     ultimately show ?thesis
     proof -
       have "\<lbrakk> \<Gamma>, n \<turnstile> (K\<^sub>1 time-delayed by \<delta>\<tau> on K\<^sub>2 implies K\<^sub>3) # \<Psi> \<triangleright> \<Phi> \<rbrakk>\<^sub>c\<^sub>o\<^sub>n\<^sub>f\<^sub>i\<^sub>g = \<lbrakk>\<lbrakk> \<Gamma> \<rbrakk>\<rbrakk>\<^sub>p\<^sub>r\<^sub>i\<^sub>m \<inter> (\<lbrakk>\<lbrakk> (K\<^sub>1 time-delayed by \<delta>\<tau> on K\<^sub>2 implies K\<^sub>3) # \<Psi> \<rbrakk>\<rbrakk>\<^sub>T\<^sub>E\<^sub>S\<^sub>L\<^bsup>\<ge> n\<^esup> \<inter> \<lbrakk>\<lbrakk> \<Phi> \<rbrakk>\<rbrakk>\<^sub>T\<^sub>E\<^sub>S\<^sub>L\<^bsup>\<ge> Suc n\<^esup>)"
         using \<open>\<lbrakk> \<Gamma>, n \<turnstile> (K\<^sub>1 time-delayed by \<delta>\<tau> on K\<^sub>2 implies K\<^sub>3) # \<Psi> \<triangleright> \<Phi> \<rbrakk>\<^sub>c\<^sub>o\<^sub>n\<^sub>f\<^sub>i\<^sub>g = \<lbrakk>\<lbrakk> \<Gamma> \<rbrakk>\<rbrakk>\<^sub>p\<^sub>r\<^sub>i\<^sub>m \<inter> \<lbrakk>\<lbrakk> (K\<^sub>1 time-delayed by \<delta>\<tau> on K\<^sub>2 implies K\<^sub>3) # \<Psi> \<rbrakk>\<rbrakk>\<^sub>T\<^sub>E\<^sub>S\<^sub>L\<^bsup>\<ge> n\<^esup> \<inter> \<lbrakk>\<lbrakk> \<Phi> \<rbrakk>\<rbrakk>\<^sub>T\<^sub>E\<^sub>S\<^sub>L\<^bsup>\<ge> Suc n\<^esup>\<close> by blast
-      then have "\<lbrakk> \<Gamma>, n \<turnstile> (K\<^sub>1 time-delayed by \<delta>\<tau> on K\<^sub>2 implies K\<^sub>3) # \<Psi> \<triangleright> \<Phi> \<rbrakk>\<^sub>c\<^sub>o\<^sub>n\<^sub>f\<^sub>i\<^sub>g = (\<lbrakk> K\<^sub>1 \<not>\<Up> n \<rbrakk>\<^sub>p\<^sub>r\<^sub>i\<^sub>m \<union> \<lbrakk> K\<^sub>1 \<Up> n \<rbrakk>\<^sub>p\<^sub>r\<^sub>i\<^sub>m \<inter> \<lbrakk> K\<^sub>3 sporadic \<lfloor> \<tau>\<^sub>v\<^sub>a\<^sub>r (K\<^sub>2, n) \<oplus> \<delta>\<tau> \<rfloor> on K\<^sub>2 \<rbrakk>\<^sub>T\<^sub>E\<^sub>S\<^sub>L\<^bsup>\<ge> n\<^esup>) \<inter> (\<lbrakk>\<lbrakk> \<Gamma> \<rbrakk>\<rbrakk>\<^sub>p\<^sub>r\<^sub>i\<^sub>m \<inter> (\<lbrakk>\<lbrakk> \<Psi> \<rbrakk>\<rbrakk>\<^sub>T\<^sub>E\<^sub>S\<^sub>L\<^bsup>\<ge> n\<^esup> \<inter> \<lbrakk>\<lbrakk> (K\<^sub>1 time-delayed by \<delta>\<tau> on K\<^sub>2 implies K\<^sub>3) # \<Phi> \<rbrakk>\<rbrakk>\<^sub>T\<^sub>E\<^sub>S\<^sub>L\<^bsup>\<ge> Suc n\<^esup>))"
+      then have "\<lbrakk> \<Gamma>, n \<turnstile> (K\<^sub>1 time-delayed by \<delta>\<tau> on K\<^sub>2 implies K\<^sub>3) # \<Psi> \<triangleright> \<Phi> \<rbrakk>\<^sub>c\<^sub>o\<^sub>n\<^sub>f\<^sub>i\<^sub>g = (\<lbrakk> K\<^sub>1 \<not>\<Up> n \<rbrakk>\<^sub>p\<^sub>r\<^sub>i\<^sub>m \<union> \<lbrakk> K\<^sub>1 \<Up> n \<rbrakk>\<^sub>p\<^sub>r\<^sub>i\<^sub>m \<inter> \<lbrakk> K\<^sub>3 sporadic \<lparr> \<tau>\<^sub>v\<^sub>a\<^sub>r (K\<^sub>2, n) \<oplus> \<delta>\<tau> \<rparr> on K\<^sub>2 \<rbrakk>\<^sub>T\<^sub>E\<^sub>S\<^sub>L\<^bsup>\<ge> n\<^esup>) \<inter> (\<lbrakk>\<lbrakk> \<Gamma> \<rbrakk>\<rbrakk>\<^sub>p\<^sub>r\<^sub>i\<^sub>m \<inter> (\<lbrakk>\<lbrakk> \<Psi> \<rbrakk>\<rbrakk>\<^sub>T\<^sub>E\<^sub>S\<^sub>L\<^bsup>\<ge> n\<^esup> \<inter> \<lbrakk>\<lbrakk> (K\<^sub>1 time-delayed by \<delta>\<tau> on K\<^sub>2 implies K\<^sub>3) # \<Phi> \<rbrakk>\<rbrakk>\<^sub>T\<^sub>E\<^sub>S\<^sub>L\<^bsup>\<ge> Suc n\<^esup>))"
         using TESL_interp_stepwise_timedelayed_coind_unfold TESL_interpretation_stepwise_cons_morph by blast
       then show ?thesis
         by auto
     qed
   qed
 
-lemma HeronConf_interp_stepwise_timedelayed_cases:
-  shows "\<lbrakk> \<Gamma>, n \<turnstile> ((K\<^sub>1 time-delayed by \<delta>\<tau> on K\<^sub>2 implies K\<^sub>3) # \<Psi>) \<triangleright> \<Phi> \<rbrakk>\<^sub>c\<^sub>o\<^sub>n\<^sub>f\<^sub>i\<^sub>g
-          = \<lbrakk> ((K\<^sub>1 \<not>\<Up> n) # \<Gamma>), n \<turnstile> \<Psi> \<triangleright> ((K\<^sub>1 time-delayed by \<delta>\<tau> on K\<^sub>2 implies K\<^sub>3) # \<Phi>) \<rbrakk>\<^sub>c\<^sub>o\<^sub>n\<^sub>f\<^sub>i\<^sub>g
-          \<union> \<lbrakk> ((K\<^sub>1 \<Up> n) # \<Gamma>), n \<turnstile> ((K\<^sub>3 sporadic \<lfloor>\<tau>\<^sub>v\<^sub>a\<^sub>r(K\<^sub>2, n) \<oplus> \<delta>\<tau>\<rfloor> on K\<^sub>2) # \<Psi>) \<triangleright> ((K\<^sub>1 time-delayed by \<delta>\<tau> on K\<^sub>2 implies K\<^sub>3) # \<Phi>) \<rbrakk>\<^sub>c\<^sub>o\<^sub>n\<^sub>f\<^sub>i\<^sub>g"
-  sorry
+lemma HeronConf_interp_stepwise_precedes_cases:
+  shows "\<lbrakk> \<Gamma>, n \<turnstile> ((K\<^sub>1 precedes K\<^sub>2) # \<Psi>) \<triangleright> \<Phi> \<rbrakk>\<^sub>c\<^sub>o\<^sub>n\<^sub>f\<^sub>i\<^sub>g
+          = \<lbrakk> ((\<lceil>#\<^sup>\<le> K\<^sub>2 n, #\<^sup>< K\<^sub>1 n\<rceil> \<in> (\<lambda>(x,y). x\<le>y)) # \<Gamma>), n \<turnstile> \<Psi> \<triangleright> ((K\<^sub>1 precedes K\<^sub>2) # \<Phi>) \<rbrakk>\<^sub>c\<^sub>o\<^sub>n\<^sub>f\<^sub>i\<^sub>g"
+  proof -
+    have "\<lbrakk> \<Gamma>, n \<turnstile> (K\<^sub>1 precedes K\<^sub>2) # \<Psi> \<triangleright> \<Phi> \<rbrakk>\<^sub>c\<^sub>o\<^sub>n\<^sub>f\<^sub>i\<^sub>g = \<lbrakk>\<lbrakk> \<Gamma> \<rbrakk>\<rbrakk>\<^sub>p\<^sub>r\<^sub>i\<^sub>m \<inter> \<lbrakk>\<lbrakk> (K\<^sub>1 precedes K\<^sub>2) # \<Psi> \<rbrakk>\<rbrakk>\<^sub>T\<^sub>E\<^sub>S\<^sub>L\<^bsup>\<ge> n\<^esup> \<inter> \<lbrakk>\<lbrakk> \<Phi> \<rbrakk>\<rbrakk>\<^sub>T\<^sub>E\<^sub>S\<^sub>L\<^bsup>\<ge> Suc n\<^esup>"
+      by simp
+    moreover have "\<lbrakk> ((\<lceil>#\<^sup>\<le> K\<^sub>2 n, #\<^sup>< K\<^sub>1 n\<rceil> \<in> (\<lambda>(x,y). x\<le>y)) # \<Gamma>), n \<turnstile> \<Psi> \<triangleright> ((K\<^sub>1 precedes K\<^sub>2) # \<Phi>) \<rbrakk>\<^sub>c\<^sub>o\<^sub>n\<^sub>f\<^sub>i\<^sub>g
+                      = \<lbrakk>\<lbrakk> (\<lceil>#\<^sup>\<le> K\<^sub>2 n, #\<^sup>< K\<^sub>1 n\<rceil> \<in> (\<lambda>(x,y). x\<le>y)) # \<Gamma> \<rbrakk>\<rbrakk>\<^sub>p\<^sub>r\<^sub>i\<^sub>m \<inter> \<lbrakk>\<lbrakk> \<Psi> \<rbrakk>\<rbrakk>\<^sub>T\<^sub>E\<^sub>S\<^sub>L\<^bsup>\<ge> n\<^esup> \<inter> \<lbrakk>\<lbrakk> (K\<^sub>1 precedes K\<^sub>2) # \<Phi> \<rbrakk>\<rbrakk>\<^sub>T\<^sub>E\<^sub>S\<^sub>L\<^bsup>\<ge> Suc n\<^esup>"
+      by simp
+    ultimately show ?thesis
+    proof -
+      have "\<lbrakk> \<lceil>#\<^sup>\<le> K\<^sub>2 n, #\<^sup>< K\<^sub>1 n\<rceil> \<in> (\<lambda>(x,y). x\<le>y) \<rbrakk>\<^sub>p\<^sub>r\<^sub>i\<^sub>m \<inter> \<lbrakk> K\<^sub>1 precedes K\<^sub>2 \<rbrakk>\<^sub>T\<^sub>E\<^sub>S\<^sub>L\<^bsup>\<ge> Suc n\<^esup> \<inter> \<lbrakk>\<lbrakk> \<Psi> \<rbrakk>\<rbrakk>\<^sub>T\<^sub>E\<^sub>S\<^sub>L\<^bsup>\<ge> n\<^esup> = \<lbrakk>\<lbrakk> (K\<^sub>1 precedes K\<^sub>2) # \<Psi> \<rbrakk>\<rbrakk>\<^sub>T\<^sub>E\<^sub>S\<^sub>L\<^bsup>\<ge> n\<^esup>"
+        using TESL_interp_stepwise_precedes_coind_unfold TESL_interpretation_stepwise_cons_morph by blast
+      then show ?thesis
+        by auto
+    qed
+  qed
+
+lemma HeronConf_interp_stepwise_precedes_cases':
+  shows "\<lbrakk> \<Gamma>, n \<turnstile> ((K\<^sub>1 precedes K\<^sub>2) # \<Psi>) \<triangleright> \<Phi> \<rbrakk>\<^sub>c\<^sub>o\<^sub>n\<^sub>f\<^sub>i\<^sub>g
+          = \<lbrakk> ((#\<^sup>\<le> K\<^sub>2 n \<preceq> #\<^sup>< K\<^sub>1 n) # \<Gamma>), n \<turnstile> \<Psi> \<triangleright> ((K\<^sub>1 precedes K\<^sub>2) # \<Phi>) \<rbrakk>\<^sub>c\<^sub>o\<^sub>n\<^sub>f\<^sub>i\<^sub>g"
+  oops
 
 end
