src/Hygge_Theory.thy
@@ -41,6 +41,7 @@ proof -
       using HeronConf_interp_stepwise_implies_cases HeronConf_interpretation.simps apply blast+
       using HeronConf_interp_stepwise_implies_not_cases HeronConf_interpretation.simps apply blast+
       using HeronConf_interp_stepwise_timedelayed_cases HeronConf_interpretation.simps apply blast+
+      using HeronConf_interp_stepwise_precedes_cases HeronConf_interpretation.simps apply blast+
     done
   qed
 qed
@@ -142,6 +143,12 @@ lemma complete_direct_successors:
         thus ?thesis
           using HeronConf_interp_stepwise_timedelayed_cases[of "\<Gamma>" "n" "Kmast" "\<tau>" "Kmeas" "Kslave" "\<Psi>" "\<Phi>"]
                 Cnext_solve_timedelayed[of "Kmast" "n" "\<Gamma>" "\<Psi>" "\<tau>" "Kmeas" "Kslave" "\<Phi>"] by blast
+      next
+        case (Precedes K1 K2)
+        then show ?thesis
+          using HeronConf_interp_stepwise_precedes_cases[of "\<Gamma>" "n" "K1" "K2" "\<Psi>" "\<Phi>"]
+                Cnext_solve_precedes[of "K2" "n" "K1" "\<Gamma>" "\<Psi>"  "\<Phi>"]
+          by blast
       qed
   qed
 
@@ -247,12 +254,12 @@ lemma instant_index_increase:
 *)
     next
       case (TagRelation K\<^sub>1 K\<^sub>2 R)
-      have branches: "\<lbrakk> \<Gamma>, n \<turnstile> ((tag-relation \<langle>K\<^sub>1, K\<^sub>2\<rangle> \<in> R) # \<Psi>) \<triangleright> \<Phi> \<rbrakk>\<^sub>c\<^sub>o\<^sub>n\<^sub>f\<^sub>i\<^sub>g
-          = \<lbrakk> ((\<langle>\<tau>\<^sub>v\<^sub>a\<^sub>r(K\<^sub>1, n), \<tau>\<^sub>v\<^sub>a\<^sub>r(K\<^sub>2, n)\<rangle> \<in> R) # \<Gamma>), n \<turnstile> \<Psi> \<triangleright> ((tag-relation \<langle>K\<^sub>1, K\<^sub>2\<rangle> \<in> R) # \<Phi>) \<rbrakk>\<^sub>c\<^sub>o\<^sub>n\<^sub>f\<^sub>i\<^sub>g"
+      have branches: "\<lbrakk> \<Gamma>, n \<turnstile> ((tag-relation \<lfloor>K\<^sub>1, K\<^sub>2\<rfloor> \<in> R) # \<Psi>) \<triangleright> \<Phi> \<rbrakk>\<^sub>c\<^sub>o\<^sub>n\<^sub>f\<^sub>i\<^sub>g
+          = \<lbrakk> ((\<lfloor>\<tau>\<^sub>v\<^sub>a\<^sub>r(K\<^sub>1, n), \<tau>\<^sub>v\<^sub>a\<^sub>r(K\<^sub>2, n)\<rfloor> \<in> R) # \<Gamma>), n \<turnstile> \<Psi> \<triangleright> ((tag-relation \<lfloor>K\<^sub>1, K\<^sub>2\<rfloor> \<in> R) # \<Phi>) \<rbrakk>\<^sub>c\<^sub>o\<^sub>n\<^sub>f\<^sub>i\<^sub>g"
         using HeronConf_interp_stepwise_tagrel_cases by simp
       then show ?case
         proof -
-          have "\<exists>\<Gamma>\<^sub>k \<Psi>\<^sub>k \<Phi>\<^sub>k k. ((((\<langle>\<tau>\<^sub>v\<^sub>a\<^sub>r(K\<^sub>1, n), \<tau>\<^sub>v\<^sub>a\<^sub>r(K\<^sub>2, n)\<rangle> \<in> R) # \<Gamma>), n \<turnstile> \<Psi> \<triangleright> ((tag-relation \<langle>K\<^sub>1, K\<^sub>2\<rangle> \<in> R) # \<Phi>))
+          have "\<exists>\<Gamma>\<^sub>k \<Psi>\<^sub>k \<Phi>\<^sub>k k. ((((\<lfloor>\<tau>\<^sub>v\<^sub>a\<^sub>r(K\<^sub>1, n), \<tau>\<^sub>v\<^sub>a\<^sub>r(K\<^sub>2, n)\<rfloor> \<in> R) # \<Gamma>), n \<turnstile> \<Psi> \<triangleright> ((tag-relation \<lfloor>K\<^sub>1, K\<^sub>2\<rfloor> \<in> R) # \<Phi>))
               \<hookrightarrow>\<^bsup>k\<^esup> (\<Gamma>\<^sub>k, Suc n \<turnstile> \<Psi>\<^sub>k \<triangleright> \<Phi>\<^sub>k)) \<and> \<rho> \<in> \<lbrakk> \<Gamma>\<^sub>k, Suc n \<turnstile> \<Psi>\<^sub>k \<triangleright> \<Phi>\<^sub>k \<rbrakk>\<^sub>c\<^sub>o\<^sub>n\<^sub>f\<^sub>i\<^sub>g"
             using TagRelation.prems by simp
           then show ?thesis
@@ -294,17 +301,18 @@ lemma instant_index_increase:
     next
       case (ImpliesNot K\<^sub>1 K\<^sub>2)
       then show ?case
-        sorry
+        by (metis (no_types, lifting) HeronConf_interp_stepwise_implies_not_cases UnE
+            elims_part implies_not_e1 implies_not_e2 relpowp_Suc_I2)
     next
       case (TimeDelayedBy K\<^sub>1 \<delta>\<tau> K\<^sub>2 K\<^sub>3)
       have branches: "\<lbrakk> \<Gamma>, n \<turnstile> ((K\<^sub>1 time-delayed by \<delta>\<tau> on K\<^sub>2 implies K\<^sub>3) # \<Psi>) \<triangleright> \<Phi> \<rbrakk>\<^sub>c\<^sub>o\<^sub>n\<^sub>f\<^sub>i\<^sub>g
           = \<lbrakk> ((K\<^sub>1 \<not>\<Up> n) # \<Gamma>), n \<turnstile> \<Psi> \<triangleright> ((K\<^sub>1 time-delayed by \<delta>\<tau> on K\<^sub>2 implies K\<^sub>3) # \<Phi>) \<rbrakk>\<^sub>c\<^sub>o\<^sub>n\<^sub>f\<^sub>i\<^sub>g
-          \<union> \<lbrakk> ((K\<^sub>1 \<Up> n) # \<Gamma>), n \<turnstile> ((K\<^sub>3 sporadic \<lfloor>\<tau>\<^sub>v\<^sub>a\<^sub>r(K\<^sub>2, n) \<oplus> \<delta>\<tau>\<rfloor> on K\<^sub>2) # \<Psi>) \<triangleright> ((K\<^sub>1 time-delayed by \<delta>\<tau> on K\<^sub>2 implies K\<^sub>3) # \<Phi>) \<rbrakk>\<^sub>c\<^sub>o\<^sub>n\<^sub>f\<^sub>i\<^sub>g"
+          \<union> \<lbrakk> ((K\<^sub>1 \<Up> n) # \<Gamma>), n \<turnstile> ((K\<^sub>3 sporadic \<lparr>\<tau>\<^sub>v\<^sub>a\<^sub>r(K\<^sub>2, n) \<oplus> \<delta>\<tau>\<rparr> on K\<^sub>2) # \<Psi>) \<triangleright> ((K\<^sub>1 time-delayed by \<delta>\<tau> on K\<^sub>2 implies K\<^sub>3) # \<Phi>) \<rbrakk>\<^sub>c\<^sub>o\<^sub>n\<^sub>f\<^sub>i\<^sub>g"
         using HeronConf_interp_stepwise_timedelayed_cases by simp
       have more_branches:
-                "\<lbrakk> ((K\<^sub>1 \<Up> n) # \<Gamma>), n \<turnstile> ((K\<^sub>3 sporadic \<lfloor>\<tau>\<^sub>v\<^sub>a\<^sub>r(K\<^sub>2, n) \<oplus> \<delta>\<tau>\<rfloor> on K\<^sub>2) # \<Psi>) \<triangleright> ((K\<^sub>1 time-delayed by \<delta>\<tau> on K\<^sub>2 implies K\<^sub>3) # \<Phi>) \<rbrakk>\<^sub>c\<^sub>o\<^sub>n\<^sub>f\<^sub>i\<^sub>g
-                  = \<lbrakk> ((K\<^sub>1 \<Up> n) # \<Gamma>), n \<turnstile> \<Psi> \<triangleright> ((K\<^sub>3 sporadic \<lfloor>\<tau>\<^sub>v\<^sub>a\<^sub>r(K\<^sub>2, n) \<oplus> \<delta>\<tau>\<rfloor> on K\<^sub>2) # (K\<^sub>1 time-delayed by \<delta>\<tau> on K\<^sub>2 implies K\<^sub>3) # \<Phi>) \<rbrakk>\<^sub>c\<^sub>o\<^sub>n\<^sub>f\<^sub>i\<^sub>g
-                  \<union> \<lbrakk> ((K\<^sub>3 \<Up> n) # (K\<^sub>2 \<Down> n @ \<lfloor>\<tau>\<^sub>v\<^sub>a\<^sub>r(K\<^sub>2, n) \<oplus> \<delta>\<tau>\<rfloor>) # (K\<^sub>1 \<Up> n) # \<Gamma>), n \<turnstile> \<Psi> \<triangleright> ((K\<^sub>1 time-delayed by \<delta>\<tau> on K\<^sub>2 implies K\<^sub>3) # \<Phi>) \<rbrakk>\<^sub>c\<^sub>o\<^sub>n\<^sub>f\<^sub>i\<^sub>g"
+                "\<lbrakk> ((K\<^sub>1 \<Up> n) # \<Gamma>), n \<turnstile> ((K\<^sub>3 sporadic \<lparr>\<tau>\<^sub>v\<^sub>a\<^sub>r(K\<^sub>2, n) \<oplus> \<delta>\<tau>\<rparr> on K\<^sub>2) # \<Psi>) \<triangleright> ((K\<^sub>1 time-delayed by \<delta>\<tau> on K\<^sub>2 implies K\<^sub>3) # \<Phi>) \<rbrakk>\<^sub>c\<^sub>o\<^sub>n\<^sub>f\<^sub>i\<^sub>g
+                  = \<lbrakk> ((K\<^sub>1 \<Up> n) # \<Gamma>), n \<turnstile> \<Psi> \<triangleright> ((K\<^sub>3 sporadic \<lparr>\<tau>\<^sub>v\<^sub>a\<^sub>r(K\<^sub>2, n) \<oplus> \<delta>\<tau>\<rparr> on K\<^sub>2) # (K\<^sub>1 time-delayed by \<delta>\<tau> on K\<^sub>2 implies K\<^sub>3) # \<Phi>) \<rbrakk>\<^sub>c\<^sub>o\<^sub>n\<^sub>f\<^sub>i\<^sub>g
+                  \<union> \<lbrakk> ((K\<^sub>3 \<Up> n) # (K\<^sub>2 \<Down> n @ \<lparr>\<tau>\<^sub>v\<^sub>a\<^sub>r(K\<^sub>2, n) \<oplus> \<delta>\<tau>\<rparr>) # (K\<^sub>1 \<Up> n) # \<Gamma>), n \<turnstile> \<Psi> \<triangleright> ((K\<^sub>1 time-delayed by \<delta>\<tau> on K\<^sub>2 implies K\<^sub>3) # \<Phi>) \<rbrakk>\<^sub>c\<^sub>o\<^sub>n\<^sub>f\<^sub>i\<^sub>g"
             using HeronConf_interp_stepwise_sporadicon_cases by blast
       have br1: "\<rho> \<in> \<lbrakk> ((K\<^sub>1 \<not>\<Up> n) # \<Gamma>), n \<turnstile> \<Psi> \<triangleright> ((K\<^sub>1 time-delayed by \<delta>\<tau> on K\<^sub>2 implies K\<^sub>3) # \<Phi>) \<rbrakk>\<^sub>c\<^sub>o\<^sub>n\<^sub>f\<^sub>i\<^sub>g
               \<Longrightarrow> \<exists>\<Gamma>\<^sub>k \<Psi>\<^sub>k \<Phi>\<^sub>k k.
@@ -319,26 +327,26 @@ lemma instant_index_increase:
           then show ?thesis
             by (meson elims_part relpowp_Suc_I2 timedelayed_e1)
         qed
-        moreover have br2: "\<rho> \<in> \<lbrakk> ((K\<^sub>1 \<Up> n) # \<Gamma>), n \<turnstile> \<Psi> \<triangleright> ((K\<^sub>3 sporadic \<lfloor>\<tau>\<^sub>v\<^sub>a\<^sub>r(K\<^sub>2, n) \<oplus> \<delta>\<tau>\<rfloor> on K\<^sub>2) # (K\<^sub>1 time-delayed by \<delta>\<tau> on K\<^sub>2 implies K\<^sub>3) # \<Phi>) \<rbrakk>\<^sub>c\<^sub>o\<^sub>n\<^sub>f\<^sub>i\<^sub>g
+        moreover have br2: "\<rho> \<in> \<lbrakk> ((K\<^sub>1 \<Up> n) # \<Gamma>), n \<turnstile> \<Psi> \<triangleright> ((K\<^sub>3 sporadic \<lparr>\<tau>\<^sub>v\<^sub>a\<^sub>r(K\<^sub>2, n) \<oplus> \<delta>\<tau>\<rparr> on K\<^sub>2) # (K\<^sub>1 time-delayed by \<delta>\<tau> on K\<^sub>2 implies K\<^sub>3) # \<Phi>) \<rbrakk>\<^sub>c\<^sub>o\<^sub>n\<^sub>f\<^sub>i\<^sub>g
           \<Longrightarrow> \<exists>\<Gamma>\<^sub>k \<Psi>\<^sub>k \<Phi>\<^sub>k k.
             ((\<Gamma>, n \<turnstile> ((K\<^sub>1 time-delayed by \<delta>\<tau> on K\<^sub>2 implies K\<^sub>3) # \<Psi>) \<triangleright> \<Phi>) \<hookrightarrow>\<^bsup>k\<^esup> (\<Gamma>\<^sub>k, Suc n \<turnstile> \<Psi>\<^sub>k \<triangleright> \<Phi>\<^sub>k))
            \<and> \<rho> \<in> \<lbrakk> \<Gamma>\<^sub>k, Suc n \<turnstile> \<Psi>\<^sub>k \<triangleright> \<Phi>\<^sub>k \<rbrakk>\<^sub>c\<^sub>o\<^sub>n\<^sub>f\<^sub>i\<^sub>g"
         proof -
-          assume h2: "\<rho> \<in> \<lbrakk> ((K\<^sub>1 \<Up> n) # \<Gamma>), n \<turnstile> \<Psi> \<triangleright> ((K\<^sub>3 sporadic \<lfloor>\<tau>\<^sub>v\<^sub>a\<^sub>r(K\<^sub>2, n) \<oplus> \<delta>\<tau>\<rfloor> on K\<^sub>2) # (K\<^sub>1 time-delayed by \<delta>\<tau> on K\<^sub>2 implies K\<^sub>3) # \<Phi>) \<rbrakk>\<^sub>c\<^sub>o\<^sub>n\<^sub>f\<^sub>i\<^sub>g"
-          then have "\<exists>\<Gamma>\<^sub>k \<Psi>\<^sub>k \<Phi>\<^sub>k k. ((((K\<^sub>1 \<Up> n) # \<Gamma>), n \<turnstile> \<Psi> \<triangleright> ((K\<^sub>3 sporadic \<lfloor>\<tau>\<^sub>v\<^sub>a\<^sub>r(K\<^sub>2, n) \<oplus> \<delta>\<tau>\<rfloor> on K\<^sub>2) # (K\<^sub>1 time-delayed by \<delta>\<tau> on K\<^sub>2 implies K\<^sub>3) # \<Phi>)) \<hookrightarrow>\<^bsup>k\<^esup> (\<Gamma>\<^sub>k, Suc n \<turnstile> \<Psi>\<^sub>k \<triangleright> \<Phi>\<^sub>k)) \<and> \<rho> \<in> \<lbrakk> \<Gamma>\<^sub>k, Suc n \<turnstile> \<Psi>\<^sub>k \<triangleright> \<Phi>\<^sub>k \<rbrakk>\<^sub>c\<^sub>o\<^sub>n\<^sub>f\<^sub>i\<^sub>g"
+          assume h2: "\<rho> \<in> \<lbrakk> ((K\<^sub>1 \<Up> n) # \<Gamma>), n \<turnstile> \<Psi> \<triangleright> ((K\<^sub>3 sporadic \<lparr>\<tau>\<^sub>v\<^sub>a\<^sub>r(K\<^sub>2, n) \<oplus> \<delta>\<tau>\<rparr> on K\<^sub>2) # (K\<^sub>1 time-delayed by \<delta>\<tau> on K\<^sub>2 implies K\<^sub>3) # \<Phi>) \<rbrakk>\<^sub>c\<^sub>o\<^sub>n\<^sub>f\<^sub>i\<^sub>g"
+          then have "\<exists>\<Gamma>\<^sub>k \<Psi>\<^sub>k \<Phi>\<^sub>k k. ((((K\<^sub>1 \<Up> n) # \<Gamma>), n \<turnstile> \<Psi> \<triangleright> ((K\<^sub>3 sporadic \<lparr>\<tau>\<^sub>v\<^sub>a\<^sub>r(K\<^sub>2, n) \<oplus> \<delta>\<tau>\<rparr> on K\<^sub>2) # (K\<^sub>1 time-delayed by \<delta>\<tau> on K\<^sub>2 implies K\<^sub>3) # \<Phi>)) \<hookrightarrow>\<^bsup>k\<^esup> (\<Gamma>\<^sub>k, Suc n \<turnstile> \<Psi>\<^sub>k \<triangleright> \<Phi>\<^sub>k)) \<and> \<rho> \<in> \<lbrakk> \<Gamma>\<^sub>k, Suc n \<turnstile> \<Psi>\<^sub>k \<triangleright> \<Phi>\<^sub>k \<rbrakk>\<^sub>c\<^sub>o\<^sub>n\<^sub>f\<^sub>i\<^sub>g"
             using h2 TimeDelayedBy.prems by simp
           then show ?thesis
             by (meson elims_part relpowp_Suc_I2 timedelayed_e2 sporadic_on_e1)
         qed
         moreover have br2':
-          "\<rho> \<in> \<lbrakk> ((K\<^sub>3 \<Up> n) # (K\<^sub>2 \<Down> n @ \<lfloor>\<tau>\<^sub>v\<^sub>a\<^sub>r(K\<^sub>2, n) \<oplus> \<delta>\<tau>\<rfloor>) # (K\<^sub>1 \<Up> n) # \<Gamma>), n \<turnstile> \<Psi> \<triangleright> ((K\<^sub>1 time-delayed by \<delta>\<tau> on K\<^sub>2 implies K\<^sub>3) # \<Phi>) \<rbrakk>\<^sub>c\<^sub>o\<^sub>n\<^sub>f\<^sub>i\<^sub>g
+          "\<rho> \<in> \<lbrakk> ((K\<^sub>3 \<Up> n) # (K\<^sub>2 \<Down> n @ \<lparr>\<tau>\<^sub>v\<^sub>a\<^sub>r(K\<^sub>2, n) \<oplus> \<delta>\<tau>\<rparr>) # (K\<^sub>1 \<Up> n) # \<Gamma>), n \<turnstile> \<Psi> \<triangleright> ((K\<^sub>1 time-delayed by \<delta>\<tau> on K\<^sub>2 implies K\<^sub>3) # \<Phi>) \<rbrakk>\<^sub>c\<^sub>o\<^sub>n\<^sub>f\<^sub>i\<^sub>g
             \<Longrightarrow> \<exists>\<Gamma>\<^sub>k \<Psi>\<^sub>k \<Phi>\<^sub>k k.
              ((\<Gamma>, n \<turnstile> ((K\<^sub>1 time-delayed by \<delta>\<tau> on K\<^sub>2 implies K\<^sub>3) # \<Psi>) \<triangleright> \<Phi>) \<hookrightarrow>\<^bsup>k\<^esup> (\<Gamma>\<^sub>k, Suc n \<turnstile> \<Psi>\<^sub>k \<triangleright> \<Phi>\<^sub>k))
             \<and> \<rho> \<in> \<lbrakk> \<Gamma>\<^sub>k, Suc n \<turnstile> \<Psi>\<^sub>k \<triangleright> \<Phi>\<^sub>k \<rbrakk>\<^sub>c\<^sub>o\<^sub>n\<^sub>f\<^sub>i\<^sub>g"
         proof -
-          assume h2: "\<rho> \<in> \<lbrakk> ((K\<^sub>3 \<Up> n) # (K\<^sub>2 \<Down> n @ \<lfloor>\<tau>\<^sub>v\<^sub>a\<^sub>r(K\<^sub>2, n) \<oplus> \<delta>\<tau>\<rfloor>) # (K\<^sub>1 \<Up> n) # \<Gamma>), n \<turnstile> \<Psi> \<triangleright> ((K\<^sub>1 time-delayed by \<delta>\<tau> on K\<^sub>2 implies K\<^sub>3) # \<Phi>) \<rbrakk>\<^sub>c\<^sub>o\<^sub>n\<^sub>f\<^sub>i\<^sub>g"
+          assume h2: "\<rho> \<in> \<lbrakk> ((K\<^sub>3 \<Up> n) # (K\<^sub>2 \<Down> n @ \<lparr>\<tau>\<^sub>v\<^sub>a\<^sub>r(K\<^sub>2, n) \<oplus> \<delta>\<tau>\<rparr>) # (K\<^sub>1 \<Up> n) # \<Gamma>), n \<turnstile> \<Psi> \<triangleright> ((K\<^sub>1 time-delayed by \<delta>\<tau> on K\<^sub>2 implies K\<^sub>3) # \<Phi>) \<rbrakk>\<^sub>c\<^sub>o\<^sub>n\<^sub>f\<^sub>i\<^sub>g"
           then have "\<exists>\<Gamma>\<^sub>k \<Psi>\<^sub>k \<Phi>\<^sub>k k.
-              ((((K\<^sub>3 \<Up> n) # (K\<^sub>2 \<Down> n @ \<lfloor>\<tau>\<^sub>v\<^sub>a\<^sub>r(K\<^sub>2, n) \<oplus> \<delta>\<tau>\<rfloor>) # (K\<^sub>1 \<Up> n) # \<Gamma>), n \<turnstile> \<Psi> \<triangleright> ((K\<^sub>1 time-delayed by \<delta>\<tau> on K\<^sub>2 implies K\<^sub>3) # \<Phi>)) \<hookrightarrow>\<^bsup>k\<^esup> (\<Gamma>\<^sub>k, Suc n \<turnstile> \<Psi>\<^sub>k \<triangleright> \<Phi>\<^sub>k))
+              ((((K\<^sub>3 \<Up> n) # (K\<^sub>2 \<Down> n @ \<lparr>\<tau>\<^sub>v\<^sub>a\<^sub>r(K\<^sub>2, n) \<oplus> \<delta>\<tau>\<rparr>) # (K\<^sub>1 \<Up> n) # \<Gamma>), n \<turnstile> \<Psi> \<triangleright> ((K\<^sub>1 time-delayed by \<delta>\<tau> on K\<^sub>2 implies K\<^sub>3) # \<Phi>)) \<hookrightarrow>\<^bsup>k\<^esup> (\<Gamma>\<^sub>k, Suc n \<turnstile> \<Psi>\<^sub>k \<triangleright> \<Phi>\<^sub>k))
             \<and> \<rho> \<in> \<lbrakk> \<Gamma>\<^sub>k, Suc n \<turnstile> \<Psi>\<^sub>k \<triangleright> \<Phi>\<^sub>k \<rbrakk>\<^sub>c\<^sub>o\<^sub>n\<^sub>f\<^sub>i\<^sub>g"
             using h2 TimeDelayedBy.prems by simp
           then show ?thesis
@@ -346,6 +354,11 @@ lemma instant_index_increase:
         qed
       ultimately show ?case
         using TimeDelayedBy.prems(2) by (metis UnE branches more_branches)
+    next
+      case (Precedes K\<^sub>1 K\<^sub>2)
+      then show ?case
+        by (metis (no_types, lifting) HeronConf_interp_stepwise_precedes_cases elims_part
+            precedes_e relpowp_Suc_I2)
     qed
   qed
 
@@ -368,8 +381,9 @@ lemma instant_index_increase_generalized:
              ((\<Gamma>, n \<turnstile> \<Psi> \<triangleright> \<Phi>) \<hookrightarrow>\<^bsup>k\<^esup> (\<Gamma>\<^sub>k, \<delta>k + Suc n \<turnstile> \<Psi>\<^sub>k \<triangleright> \<Phi>\<^sub>k))
             \<and> \<rho> \<in> \<lbrakk> \<Gamma>\<^sub>k, \<delta>k + Suc n \<turnstile> \<Psi>\<^sub>k \<triangleright> \<Phi>\<^sub>k \<rbrakk>\<^sub>c\<^sub>o\<^sub>n\<^sub>f\<^sub>i\<^sub>g"
           using Suc.hyps by blast
-        obtain \<Gamma>\<^sub>k \<Psi>\<^sub>k \<Phi>\<^sub>k k where cont: "((\<Gamma>, n \<turnstile> \<Psi> \<triangleright> \<Phi>) \<hookrightarrow>\<^bsup>k\<^esup> (\<Gamma>\<^sub>k, \<delta>k + Suc n \<turnstile> \<Psi>\<^sub>k \<triangleright> \<Phi>\<^sub>k)) \<and> \<rho> \<in> \<lbrakk> \<Gamma>\<^sub>k, \<delta>k + Suc n \<turnstile> \<Psi>\<^sub>k \<triangleright> \<Phi>\<^sub>k \<rbrakk>\<^sub>c\<^sub>o\<^sub>n\<^sub>f\<^sub>i\<^sub>g" using f0 assms(1)
-          using Suc.prems by blast
+        obtain \<Gamma>\<^sub>k \<Psi>\<^sub>k \<Phi>\<^sub>k k
+          where cont: "((\<Gamma>, n \<turnstile> \<Psi> \<triangleright> \<Phi>) \<hookrightarrow>\<^bsup>k\<^esup> (\<Gamma>\<^sub>k, \<delta>k + Suc n \<turnstile> \<Psi>\<^sub>k \<triangleright> \<Phi>\<^sub>k)) \<and> \<rho> \<in> \<lbrakk> \<Gamma>\<^sub>k, \<delta>k + Suc n \<turnstile> \<Psi>\<^sub>k \<triangleright> \<Phi>\<^sub>k \<rbrakk>\<^sub>c\<^sub>o\<^sub>n\<^sub>f\<^sub>i\<^sub>g"
+          using f0 assms(1) Suc.prems by blast
         then have fcontinue: "\<exists>\<Gamma>\<^sub>k' \<Psi>\<^sub>k' \<Phi>\<^sub>k' k'. ((\<Gamma>\<^sub>k, \<delta>k + Suc n \<turnstile> \<Psi>\<^sub>k \<triangleright> \<Phi>\<^sub>k) \<hookrightarrow>\<^bsup>k'\<^esup> (\<Gamma>\<^sub>k', Suc (\<delta>k + Suc n) \<turnstile> \<Psi>\<^sub>k' \<triangleright> \<Phi>\<^sub>k'))
                                               \<and> \<rho> \<in> \<lbrakk> \<Gamma>\<^sub>k', Suc (\<delta>k + Suc n) \<turnstile> \<Psi>\<^sub>k' \<triangleright> \<Phi>\<^sub>k' \<rbrakk>\<^sub>c\<^sub>o\<^sub>n\<^sub>f\<^sub>i\<^sub>g"
           using f0 cont instant_index_increase by blast
@@ -441,6 +455,5 @@ theorem instant_computation_termination:
         by simp
     qed
   qed
-
 
 end
